Mica/SeparationLogic.lean
@@ -1,3 +1,4 @@
 import Mica.SeparationLogic.Axioms
 import Mica.SeparationLogic.SpatialAtom
 import Mica.SeparationLogic.Interpretations
+import Mica.SeparationLogic.PrimitiveLaws
